## 1991-AL-P MATH 1 #01
$\begin{vmatrix}
a^3 & b^3 & c^3\\
a & b & c\\
1 & 1 & 1
\end{vmatrix} = \begin{vmatrix}
1 & 1 & 1\\ 
a^3 & b^3 & c^3\\
a & b & c
\end{vmatrix} = \begin{vmatrix}
1 & 1 & 1\\ 
0 & b^3-a^3 & c^3-a^3\\
0 & b-a & c-a
\end{vmatrix}$

$= \begin{vmatrix}
b^3-a^3 & c^3-a^3\\
b-a & c-a
\end{vmatrix}$

$=(b^3-a^3)(c-a) - (c^3-a^3)(b-a)$
$=(b-a)(b^2+ab+a^2)(c-a) - (c-a)(c^2+ac+a^2)(b-a)$
$=(b-a)(c-a)(b^2+ab+a^2-c^2-ac-a^2)$
$=(b-a)(c-a)(b^2+ab-c^2-ac)$
$=(b-a)(c-a)(b^2-c^2+ab-ac)$
$=(b-a)(c-a)[(b-c)(b+c)+a(b-c)]$
$=(b-a)(c-a)(b-c)(a+b+c)$
