For any $\Delta \in R$,
$\displaystyle f(x+\Delta)-f(x)$

$\displaystyle = {1 \over {1+x+\Delta}} -  {1 \over {1+x}}$

$\displaystyle = {{(1+x) - (1+x+\Delta)} \over {(1+x+\Delta)(1+x)}}$

$\displaystyle = {{-\Delta} \over {(1+x+\Delta)(1+x)}}$

Therefore,
$\displaystyle f^{\ '}(x) = \lim_{\Delta \rightarrow 0} {{f(x+\Delta)-f(x)} \over \Delta}$

$\displaystyle = \lim_{\Delta \rightarrow 0} {{-\Delta} \over {(1+x+\Delta)(1+x)}} \cdot {1 \over \Delta}$

$\displaystyle = \lim_{\Delta \rightarrow 0} {{-1} \over {(1+x+\Delta)(1+x)}}$

$\displaystyle = {{-1} \over {(1+x)(1+x)}}$

$\displaystyle = {{-1} \over {(1+x)^2}}$

