## 1(a)
$(\sqrt{2(x+\Delta x)} - \sqrt{2x}) (\sqrt{2(x+\Delta x)}) + \sqrt{2x})$ 
$= (\sqrt{2(x+\Delta x)})^2 - (\sqrt{2x})^2$
$= 2(x+\Delta x) - 2x$
$= 2\Delta x$

## 1(b)
$\displaystyle {d \over {dx}} (\sqrt{2x})$
$\displaystyle = \lim_{\Delta x \rightarrow 0} {{\sqrt{2(x+\Delta x)} - \sqrt{2x}} \over \Delta x}$

$\displaystyle = \lim_{\Delta x \rightarrow 0} {{(\sqrt{2(x+\Delta x)} - \sqrt{2x}) (\sqrt{2(x+\Delta x)}) + \sqrt{2x})} \over {\Delta x (\sqrt{2(x+\Delta x)}) + \sqrt{2x})}}$

$\displaystyle = \lim_{\Delta x \rightarrow 0} {{2\Delta x} \over {\Delta x (\sqrt{2(x+\Delta x)}) + \sqrt{2x})}}$

$\displaystyle = \lim_{\Delta x \rightarrow 0} {{\sqrt{2}} \over { \sqrt{(x+\Delta x)}) + \sqrt{x}}}$

$\displaystyle = {{\sqrt{2}} \over {2\sqrt{x}}}$

$\displaystyle = {1 \over {\sqrt{2x}}}$