$\displaystyle y = tan({1 \over x})$

$\displaystyle \Rightarrow {{dy} \over {dx}} = sec^2({1 \over x}) \cdot { d \over {dx}} ({1 \over x})$

$\displaystyle \Rightarrow {{dy} \over {dx}} = - {1 \over {x^2}} \cdot sec^2({1 \over x})$

Therefore,
$\displaystyle x^2{{dy} \over {dx}} + y^2 + 1$

$\displaystyle = - {1 \over {x^2}} \cdot sec^2({1 \over x}) \cdot x^2 + tan^2({1 \over x}) + 1$

$\displaystyle = - sec^2({1 \over x}) + sec^2({1 \over x})-1 + 1$
$= 0$

-----
$\displaystyle x^2{{dy} \over {dx}} + y^2 + 1 = 0$

$\displaystyle \Rightarrow {d \over {dx}} [\ x^2{{dy} \over {dx}} + y^2 + 1\ ] = 0$

$\displaystyle \Rightarrow {d \over {dx}}(x^2{{dy} \over {dx}}) + {d \over {dx}}(y^2) + {d \over {dx}}(1) = 0$

$\displaystyle \Rightarrow 2x{{dy} \over {dx}} + x^2{{d^2y} \over {dx^2}} + 2y{{dy} \over {dx}} = 0$

$\displaystyle \Rightarrow x^2{{d^2y} \over {dx^2}} + 2x{{dy} \over {dx}} + 2y{{dy} \over {dx}} = 0$

$\displaystyle \Rightarrow x^2{{d^2y} \over {dx^2}} + 2(x+y){{dy} \over {dx}} = 0$

$\displaystyle \Rightarrow {{d^2y} \over {dx^2}} + {2(x+y) \over {x^2}} {{dy} \over {dx}} = 0$