
## 1996-AL-P MATH 1 #01
$A^3 - 5A^2 + 8A - 4I = (A - I) (A - 2I)^2$
 $\displaystyle \Rightarrow A^3 - 5A^2 + 8A - 4I = (A - I) (A - 2I)^2 = \begin{pmatrix}
-1 & 0 & -2 \\
1 & 1 & 1 \\
1 & 0 & 2
\end{pmatrix} \begin{pmatrix}
-2 & 0 & -2 \\
1 & 0 & 1 \\
1 & 0 & 1
\end{pmatrix} \begin{pmatrix}
-2 & 0 & -2 \\
1 & 0 & 1 \\
1 & 0 & 1
\end{pmatrix}$

 $\displaystyle \Rightarrow A^3 - 5A^2 + 8A - 4I = \begin{pmatrix}
-1 & 0 & -2 \\
1 & 1 & 1 \\
1 & 0 & 2
\end{pmatrix} \begin{pmatrix}
-2 & 0 & -2 \\
1 & 0 & 1 \\
1 & 0 & 1
\end{pmatrix} \begin{pmatrix}
-2 & 0 & -2 \\
1 & 0 & 1 \\
1 & 0 & 1
\end{pmatrix}$

 $\displaystyle \Rightarrow A^3 - 5A^2 + 8A - 4I = \begin{pmatrix}
0 & 0 & 0 \\
0 & 0 & 0 \\
0 & 0 & 0
\end{pmatrix} \begin{pmatrix}
-2 & 0 & -2 \\
1 & 0 & 1 \\
1 & 0 & 1
\end{pmatrix}$

$\displaystyle \Rightarrow A^3 - 5A^2 + 8A - 4I = 0$

Hence, 
$\displaystyle 4I = A^3 - 5A^2 + 8A$
$\displaystyle \Rightarrow 4 A^{-1} = A^2 - 5A + 8I$
$\displaystyle \Rightarrow 4 A^{-1} = \begin{pmatrix}
0 & 0 & -2 \\
1 & 2 & 1 \\
1 & 0 & 3
\end{pmatrix} \begin{pmatrix}
0 & 0 & -2 \\
1 & 2 & 1 \\
1 & 0 & 3
\end{pmatrix} - 5 \begin{pmatrix}
0 & 0 & -2 \\
1 & 2 & 1 \\
1 & 0 & 3
\end{pmatrix} + \begin{pmatrix}
8 & 0 & 0 \\
0 & 8 & 0 \\
0 & 0 & 8
\end{pmatrix}$

$\displaystyle \Rightarrow 4 A^{-1} = \begin{pmatrix}
-2 & 0 & -6 \\
3 & 4 & 3 \\
3 & 0 & 7
\end{pmatrix} - \begin{pmatrix}
0 & 0 & -10 \\
5 & 10 & 5 \\
5 & 0 & 15
\end{pmatrix} + \begin{pmatrix}
8 & 0 & 0 \\
0 & 8 & 0 \\
0 & 0 & 8
\end{pmatrix}$

$\displaystyle \Rightarrow 4 A^{-1} = \begin{pmatrix}
6 & 0 & 4 \\
-2 & 2 & -2 \\
-2 & 0 & 0
\end{pmatrix}$

$\displaystyle \Rightarrow A^{-1} = {1 \over 2} \begin{pmatrix}
3 & 0 & 2 \\
-1 & 1 & -1 \\
-1 & 0 & 0
\end{pmatrix}$
