$\displaystyle {d \over {dx}} (\sqrt{x})$
$\displaystyle = \lim_{\Delta x \rightarrow 0} {{\sqrt{(x+\Delta x)} - \sqrt{x}} \over \Delta x}$

$\displaystyle = \lim_{\Delta x \rightarrow 0} {{(\sqrt{(x+\Delta x)} - \sqrt{x}) (\sqrt{(x+\Delta x)}) + \sqrt{x})} \over {\Delta x (\sqrt{(x+\Delta x)}) + \sqrt{x})}}$

$\displaystyle = \lim_{\Delta x \rightarrow 0} {{(\sqrt{(x+\Delta x)})^2 - (\sqrt{x})^2} \over {\Delta x (\sqrt{(x+\Delta x)}) + \sqrt{x})}}$

$\displaystyle = \lim_{\Delta x \rightarrow 0} {{x+\Delta x - x} \over {\Delta x (\sqrt{(x+\Delta x)}) + \sqrt{x})}}$

$\displaystyle = \lim_{\Delta x \rightarrow 0} {{\Delta x} \over {\Delta x (\sqrt{(x+\Delta x)}) + \sqrt{x})}}$

$\displaystyle = \lim_{\Delta x \rightarrow 0} {1 \over {\sqrt{(x+\Delta x)}) + \sqrt{x}}}$

$\displaystyle = {1 \over {2\sqrt{x}}}$