## 2(a)
$P(x)$
$= (x+\lambda)(x+\lambda)^2(x+\lambda)^3 + 12 - 15(x+\lambda) - 8(x+\lambda)^2$
$= (x+\lambda)^6 + 12 - 15(x+\lambda) - 8(x+\lambda)^2$

Therefore, 
Coefficient of $\displaystyle x^3 = \binom{6}{3}\lambda^3$
$\displaystyle \Rightarrow 20\lambda^3 = 160$
$\displaystyle \Rightarrow \lambda^3 = 8$
$\displaystyle \Rightarrow \lambda = 2$

## 2(b)
$P(x) = (x+\lambda)^6 + 12 - 15(x+\lambda) - 8(x+\lambda)^2$
$\Rightarrow P^{'}(x) = 6(x+\lambda)^5 - 15 - 16(x+\lambda)$
$\Rightarrow P^{'}(0) = 6\lambda^5 - 15 - 16\lambda$
$\Rightarrow P^{'}(0) = 6(2)^5 - 15 - 16(2)$
$\Rightarrow P^{'}(0) = 192 - 15 - 32 = 145$