# (i)
$\displaystyle {2 \over {x^2-1}} \equiv {a \over {x-1}} + {b \over {x+1}}$

$\displaystyle \Rightarrow 2 = a(x+1)+b(x-1)$
$\displaystyle \Rightarrow (a+b)x + a-b = 2$

$\Rightarrow \begin{cases}
a+b=0 \\
a-b = 2
\end{cases}$

$\Rightarrow a=1$, $b=-1$

# (ii)

A = (2, $\displaystyle {7 \over 3}$) and B = (3, $\displaystyle {3 \over 2}$)

Equation of line joining AB is:
$\displaystyle {{y-{3 \over 2}} \over {x-3}}={{{3 \over 2}-{7 \over 3}} \over {3-2}}$

$\displaystyle \Rightarrow {{y-{3 \over 2}} \over {x-3}}=-{5 \over 6}$

$\displaystyle \Rightarrow y=-{5 \over 6}(x-3)+{3 \over 2}$

$\displaystyle \Rightarrow y=-{5 \over 6}x+4$

-----
Note that:
$\displaystyle f(x) = {{x^2 + 3} \over {x^2-1}}=1+{4 \over {x^2-1}}=1+{2 \over {x-1}} - {2 \over {x+1}}$ 

Area = $\displaystyle \int_{2}^{3} [\ -{5 \over 6}x+4 - f(x)\ ]dx$

$\displaystyle = \int_{2}^{3} [\ -{5 \over 6}x+3 - {2 \over {x-1}} + {2 \over {x+1}} ]dx$

$\displaystyle = [\ -{5 \over 12}x^2+3x - 2\ ln(x-1) + 2\ ln(x+1)\ ]^3_2$

$\displaystyle = [\ -{5 \over 12}x^2+3x + 2\ ln({{x+1} \over {x-1}})\ ]^3_2$

$\displaystyle =  -{25 \over 12}+3 + 2\ ln({2 \over 3})$

$\displaystyle =  {11 \over 12} - 2\ ln({3 \over 2})$

$\displaystyle \approx 0.1057$